
\begin{proof}
    By the triangle inequality,
    \begin{equation*}
        \abs{\exp{u} - \sum_{k=0}^l \frac{v^k}{k!}} \leq \abs{\exp{u} - \exp{v}} + \abs{\sum_{k=l+1}^\infty \frac{v^k}{k!}}.
    \end{equation*}
    Starting with the second term on the right hand side, we have
    \begin{align*}
        \abs{\sum_{k=l+1}^\infty \frac{v^k}{k!}} 
        & \leq \sum_{k=l+1}^\infty \abs{\frac{v^k}{k!}} 
        = \abs{\frac{v^{l+1}}{(l+1)!}} \sum_{k=0}^\infty \abs{v^k} \frac{(l+1)!}{(k + l + 1)!} \\
        & \leq \abs{\frac{v^{l+1}}{(l+1)!}} \sum_{k=0}^\infty \abs{\frac{v^k}{k!}}
        = \abs{\frac{v^{l+1}}{(l+1)!}} \exp v\\
        &\leq \abs{\frac{v^{l+1}}{(l+1)!}} \max \left\{ \exp{|u|}, \exp{|v|} \right\}.
    \end{align*}
    Furthermore, by Taylor's theorem there exists a point $z \in \C$ lying on the straight line between $u$ and $v$ such that
    \begin{equation*}
        \exp u - \exp v = \abs{u - v} \exp z.
    \end{equation*}
    Taking absolute values and by convexity of the exponential function, we find the following bound
    \begin{equation*}
        \abs{\exp u - \exp v} = \abs{u - v} \exp |z| \leq \abs{u - v} \max \left\{ \exp{|u|}, \exp{|v|} \right\}.
    \end{equation*}
    Combining the two bounds found previously completes the proof of the lemma.
\end{proof}